add ml file

code/rocq/ml/bin/main.ml
@@ -1,0 +1,37 @@
+
+open Ml.Src
+open Unif
+open Language
+
+let rec fromn = function
+  | 0 -> O
+  | x -> S (fromn (x-1))
+
+let xA = Data (fromn 0)
+let xB = Data (fromn 1)
+let xC = Data (fromn 2)
+let xD = Data (fromn 3)
+let xE = Data (fromn 4)
+
+let s = fun _ -> None
+
+
+let p : program = { rules = []; modes = (fun _ -> []) ; coq_sig = fun _ -> Coq_b Exp }
+let f x = (Goal (p, (Call x)))
+
+
+let _ =
+  let s = state_to_list 
+    (And ((Or (OK, s, (f xB))), (f xC), (And ((Or ((Goal (p, Cut)), s, (f xD))), (f xE), (Goal (p, Cut))))))  [] in
+  Format.eprintf "%a@." pp_alts s
+
+
+(* 
+  (* (OK \/_{s1} B) /\_C ((! \/_{s2} D) /\_{E} !) *)
+  state_to_list 
+    (And (Or OK s1 (f B)) (f C) (And (Or (Goal p Cut) s2 (f D)) (f E) (Goal p Cut))) [::] = 
+    [:: 
+      [:: cut [:: [:: call p B; call p C]]; cut [::]];
+      [:: call p D; call p E]; 
+      [:: call p B; call p C]].
+ *)
