code/rocq/lang.v
@@ -88,4 +88,193 @@ Module Type Unif.
   Import Language.
   Parameter unify : Tm -> Tm -> Sigma -> option Sigma.
   Parameter matching : Tm -> Tm -> Sigma -> option Sigma.
+
+    Inductive state :=
+    | Bot : state
+    | OK : state
+    | Top : state
+    | Dead : state
+    | Goal : program  -> A -> state
+    | Or  : state -> Sigma -> state -> state  (* Or A s B := A is lhs, B is rhs, s is the subst from which launch B *)
+    | And : state -> state -> state -> state  (* And A B0 B := A is lhs, B is rhs, B0 to reset B for backtracking *)
+    .
+
+  Inductive G := 
+    | call : program -> Tm -> G
+    | cut : list (list G) -> G
+    .
+
+  Definition if_cut F g :=
+    match g with
+    | cut a => F a
+    | _ => true
+    end.
+
+  Definition apply_cut F g :=
+    match g with
+    | cut a => cut (F a) 
+    | _ => g
+    end.
+
+
+  Definition alt := (list G).
+
+  Definition a2g p A :=
+    match A with
+    | Cut => cut [::]
+    | Call t => call p t
+    end.
+
+  Definition a2gs p (b : Sigma * R) :=
+    map (a2g p) b.2.(premises).
+
+  Section add_ca.
+
+    Definition add_ca alts a :=
+      match a with
+      | cut a1 => cut (a1 ++ alts)
+      | call pr t => call pr t
+      end.
+
+    Lemma add_ca_empty {lA}:
+      map (add_ca [::]) lA = lA.
+    Proof.
+      rewrite /add_ca; elim: lA => //= x xs IH.
+      rewrite IH; case: x => // l; rewrite cats0//if_same//.
+    Qed.
+
+    Lemma map_add0_cas_empty {lA}:
+      map (map (add_ca [::])) lA  = lA.
+    Proof.
+      rewrite /add_ca; elim: lA => //= x xs ->.
+      f_equal; apply add_ca_empty.
+    Qed.
+  End add_ca.
+
+
+  Definition save_alt a gs b := map (add_ca a) b ++ gs.
+  Definition more_alt a bs gs := map (save_alt a gs) bs ++ a.
+  Definition get_ca g :=
+    match g with
+    | cut a => a 
+    | _ => [::]
+    end.
+
+  Definition is_cutb' A := match A with cut _ => true | _ => false end.
+  Definition cuts' A := all is_cutb' A.
+
+  Lemma cuts_cat {x y} : cuts' (x ++ y) = cuts' x && cuts' y.
+  Proof. rewrite/cuts' all_cat//. Qed.
+
+  Fixpoint add_ca_deep n tl (alts: seq (seq G)) := (*always:= adds always alts to cut *)
+    match n with
+    | 0 => alts
+    | n.+1 => map (map (fun x => (add_ca tl (apply_cut (add_ca_deep n tl) x)))) alts
+    end.
+
+  (* Definition add_ca1 tl a := add_ca_deep (size a) tl a. *)
+
+  Lemma add_ca_empty1 l: add_ca [::] l = l.
+  Proof. case: l => //= l1; rewrite cats0//. Qed.
+
+  Lemma map_add1_cas_empty {T: Type} (lA: list (list T)) F:
+    map (map (fun x => add_ca [::] (F x))) lA  = map (map F) lA.
+  Proof.
+    rewrite /add_ca; elim: lA => //= x xs ->.
+    f_equal; elim: x => //=x {}xs->; case: (F x)=>//=l; rewrite cats0//.
+  Qed.
+
+  Lemma cut_add_ca {l x}: is_cutb' (add_ca l x) = is_cutb' x.
+  Proof. case: x => //=*. Qed.
+
+  Lemma cuts_add_ca {x l} : cuts' [seq add_ca l j | j <- x] = cuts' x.
+  Proof. elim: x l => // x xs H/= l; rewrite H cut_add_ca//. Qed.
+
+  Definition add_suff (bt: seq alt) hd (l:seq alt) :=
+    let s := size l - size bt in
+    map (fun x => x ++ hd) (take s l) ++ drop s l.
+
+  Definition add_deep_help add_deep bt (n:nat) hd :=
+    apply_cut (fun x => add_suff bt hd (add_deep bt n hd x)).
+
+  Fixpoint add_deep bt n (l: alt) (A: seq alt) :=
+    match n with
+    | 0 => A
+    | n.+1 =>
+      map (map (add_deep_help add_deep bt n l)) A
+    end. 
+
+  Definition add_deep_ bt n (l: alt) (A: alt) :=
+    match n with
+    | 0 => A
+    | n.+1 => (map (add_deep_help add_deep bt n l)) A
+    end.
+
+  Definition kill (A: alt) := map (apply_cut (fun x => [::])) A.
+
+  Definition make_lB0 (xs:seq alt) (lB0: alt) := map (fun x => x ++ lB0) xs.
+
+    (* bt is the backtracking list for the cut-alternatives
+      this list is important since in this tree:
+           or   
+          /  \  
+         or   K 
+        /  \    
+       !    J   
+      K is in bt but not J, i.e. we have to consider two different levels:
+      the "siblings" on the right of a cut are NOT alternatives
+      the "great^n uncles" on the right of a cut ARE alternatives
+    *)
+
+  Fixpoint state_to_list (A: state) (bt : list alt) : list alt :=
+    match A with
+    | OK => [::[::]]
+    | Top => [::[::]]
+    | Bot => [::]
+    | Dead => [::]
+    | Goal _ Cut => [::[::cut [::]]]
+    | Goal pr (Call t) => [::[::call pr t]]
+    | Or A _ B => 
+      let lB := state_to_list B [::] in
+      let lA := state_to_list A lB in
+      add_ca_deep (size (lA ++ lB)) bt (lA ++ lB)
+    | And A B0 B =>
+      let lB0 := state_to_list B0 bt in
+      let lA   := state_to_list A bt in
+      if lA is x :: xs then 
+        (* lA is split into the current goal x and the future alternatives xs *)
+        (* in a valid state lB0 has length 0 or 1 (it is a (potentially killed) base and) *)
+        match lB0 with
+        | [::] => 
+          (* the reset point is empty: it kill all the alternatives in the cut-to *)
+          let lB   := state_to_list B bt in
+          [seq (kill x) ++ y | y <- lB]
+        | [::hd] =>
+        (* 
+          invariant every cut-to has bt has tail or is empty
+        *)
+          (* the reset point exists, it has to be added to all cut-to alternatives *)
+          let x := add_deep_ bt (size xs).+1 hd x in
+          let xs := add_deep bt (size xs) hd xs in 
+          (* each alt in xs must have hd has rightmost conjunct  *)
+          let xs := make_lB0 xs hd in
+          (* xs are alternatives that should be added in the deep cuts in B *)
+          let lB   := state_to_list B (xs ++ bt) in
+          (* lB are alternatives, each of them have x has head *)
+          [seq x ++ y | y <- lB] ++ xs
+        | _ => [::] (*unreachable in a valid_state*)
+        end
+      else [::]
+    end.
+
+    Require Import Extraction.
+    Extract Inductive unit => "unit" [ "()" ].
+    Extract Inductive bool => "bool" [ "true" "false" ].
+    Extract Inductive sumbool => "bool" [ "true" "false" ].
+    Extract Inductive list => "list" [ "[]" "(::)" ].
+    Extract Inductive prod => "(*)"  [ "(,)" ].
+    Extract Inductive option => "option"  [ "None" "Some" ].
+    Extraction "code.ml" state_to_list.
 End Unif.
+
+
